theories_eval/LevelZero.v
@@ -1,0 +1,425 @@
+From Prototype Require Import Prelude Sig LevelOne LevelTwo LevelTwoIrred LevelTwoSimp.
+Module P := Prelude.
+
+(** Concrete terms, renamings and substitutions. *)
+
+Inductive term :=
+| Var : nat -> term
+| App : term -> term -> term 
+| Lam : string -> term -> term.
+
+Fixpoint rename (t : term) (r : nat -> nat) : term :=
+  match t with 
+  | Var i => Var (r i)
+  | App t1 t2 => App (rename t1 r) (rename t2 r)
+  | Lam str t => Lam str (rename t (up_ren r))
+  end.
+
+Definition subst := nat -> term.
+
+Definition srcomp (s : subst) (r : ren) : subst :=
+  fun i => rename (s i) r.
+  
+Definition rscomp (r : ren) (s : subst) : subst :=
+  fun i => s (r i).
+
+Definition sid : subst :=
+  fun i => Var i.
+
+Definition sshift : subst :=
+  fun i => Var (S i).
+
+Definition scons (t : term) (s : subst) : subst :=
+  fun i => match i with 0 => t | S i => s i end.
+
+Definition up_subst (s : subst) : subst :=
+  scons (Var 0) (srcomp s rshift).
+
+Fixpoint substitute (t : term) (s : subst) : term :=
+  match t with 
+  | Var i => s i
+  | App t1 t2 => App (substitute t1 s) (substitute t2 s)
+  | Lam str t => Lam str (substitute t (up_subst s))
+  end.
+
+Definition scomp (s1 s2 : subst) : subst :=
+  fun i => substitute (s1 i) s2.
+
+(** Congruence lemmas. *)
+
+Lemma congr_app {t1 t1' t2 t2'} :
+  t1 = t1' -> t2 = t2' -> App t1 t2 = App t1' t2'.
+Proof. intros -> ->. reflexivity. Qed.
+
+Lemma congr_lam str {t t'} :
+  t = t' -> Lam str t = Lam str t'.
+Proof. intros ->. reflexivity. Qed.
+
+Lemma congr_rcons i {r r'} :
+  r =₁ r' -> P.rcons i r =₁ P.rcons i r'.
+Proof. intros H [|i'] ; [reflexivity|]. now simp rcons. Qed.
+
+Lemma congr_rcomp {r1 r1' r2 r2'} :
+  r1 =₁ r1' -> r2 =₁ r2' -> rcomp r1 r2 =₁ rcomp r1' r2'.
+Proof. intros H1 H2 i. simp rcomp. now rewrite H1, H2. Qed.
+
+Lemma congr_up_ren {r r'} :
+  r =₁ r' -> up_ren r =₁ up_ren r'.
+Proof. intros H. simp up_ren. apply congr_rcons. now apply congr_rcomp. Qed.
+
+Lemma congr_rename {t t' r r'} :
+  t = t' -> r =₁ r' -> rename t r = rename t' r'.
+Proof. 
+intros <-. revert r r'. induction t ; intros r r' H ; simpl ; auto.
+- now erewrite IHt1, IHt2.
+- rewrite (IHt (up_ren r) (up_ren r')).
+  + reflexivity.
+  + now apply congr_up_ren.
+Qed. 
+
+Lemma congr_rscomp {r r' s s'} :
+  r =₁ r' -> s =₁ s' -> rscomp r s =₁ rscomp r' s'.
+Proof. intros H1 H2 i. cbv [rscomp]. now rewrite H1, H2. Qed.
+
+Lemma congr_srcomp {s s' r r'} :
+  s =₁ s' -> r =₁ r' -> srcomp s r =₁ srcomp s' r'.
+Proof. intros H1 H2 i. cbv [srcomp]. apply congr_rename ; auto. Qed.
+
+Lemma congr_scons {t t' s s'} : 
+  t = t' -> s =₁ s' -> scons t s =₁ scons t' s'.
+Proof. intros -> H [|i] ; [reflexivity|]. simpl. apply H. Qed.
+
+Lemma congr_up_subst {s s'} :
+  s =₁ s' -> up_subst s =₁ up_subst s'.
+Proof. 
+intros H. unfold up_subst. apply congr_scons ; auto. 
+now apply congr_srcomp. 
+Qed.
+
+Lemma congr_substitute {t t' s s'} :
+  t = t' -> s =₁ s' -> substitute t s = substitute t' s'.
+Proof. 
+intros <-. revert s s'. induction t ; intros s0 s0' H ; simpl ; auto.
+- now erewrite IHt1, IHt2. 
+- f_equal. apply IHt. now apply congr_up_subst.
+Qed.
+
+Lemma congr_scomp {s1 s1' s2 s2'} :
+  s1 =₁ s1' -> s2 =₁ s2' -> scomp s1 s2 =₁ scomp s1' s2'.
+Proof. intros H1 H2 i. cbv [scomp]. now apply congr_substitute. Qed.
+
+(** Signature. *)
+
+Inductive base := BString.
+Definition denote_base (b : base) : Type := 
+  match b with BString => string end.
+
+Inductive ctor := CApp | CLam.
+Definition ctor_type c : list (@arg_ty base) := 
+  match c with 
+  | CApp => [ AT_term ; AT_term ]
+  | CLam => [ AT_base BString ; AT_bind AT_term ]
+  end.
+
+Module S.
+Definition t := Build_signature base denote_base ctor ctor_type.
+End S.
+
+Module T := LevelTwoSimp.Make (S).
+Module O := T.T.T.O.
+
+(** Custom induction principle on level one terms. *)
+
+(** Size of a level one expression. This is needed to prove a custom 
+    induction principle for level one terms. *)
+Equations esize {k} : O.expr k -> nat :=
+esize (O.E_var _) := 0 ;
+esize (O.E_ctor c al) := S (esize al) ;
+esize O.E_al_nil := 0 ;
+esize (O.E_al_cons a al) := S (esize a + esize al) ;
+esize (O.E_abase _ _) := 0 ;
+esize (O.E_aterm t) := S (esize t) ;
+esize (O.E_abind a) := S (esize a).
+
+Section TermInd.
+  Context (P : O.expr Kt -> Prop).
+  Context (H1 : forall i, P (O.E_var i)).
+  Context (H2 : forall t1 t2, P t1 -> P t2 -> 
+      P (O.E_ctor CApp (O.E_al_cons (O.E_aterm t1) (O.E_al_cons (O.E_aterm t2) O.E_al_nil)))).
+  Context (H3 : forall str t, P t -> 
+      P (O.E_ctor CLam (O.E_al_cons (O.E_abase BString str) (O.E_al_cons (O.E_abind (O.E_aterm t)) O.E_al_nil)))).
+
+  Lemma term_ind' : forall t, P t.
+  Proof.  
+  apply PeanoNat.Nat.measure_induction with (f := esize).
+  intros t IH. depelim t.
+  - now apply H1.
+  - depelim c ; simpl in *.
+    + depelim t. depelim t1. depelim t2. depelim t2_1. depelim t2_2.
+      apply H2 ; apply IH ; repeat (simp esize ; simpl) ; lia.
+    + depelim t. depelim t1. depelim t2. depelim t2_1. depelim t2_2. depelim t2_1.
+      apply H3. apply IH. repeat (simp esize ; simpl). lia.
+  Qed.
+End TermInd. 
+
+(** Reification/evaluation functions. *)
+
+Fixpoint reify (t : term) : O.expr Kt :=
+  match t with
+  | Var i => O.E_var i
+  | App t1 t2 =>
+    O.E_ctor CApp 
+      (O.E_al_cons (O.E_aterm (reify t1))
+      (O.E_al_cons (O.E_aterm (reify t2))
+       O.E_al_nil))
+  | Lam str t =>
+    O.E_ctor CLam 
+      (O.E_al_cons (O.E_abase BString str)
+      (O.E_al_cons (O.E_abind (O.E_aterm (reify t)))
+       O.E_al_nil))
+  end.
+
+Definition sreify (s : subst) : O.subst :=
+  fun i => reify (s i).
+  
+Fixpoint eval_arg (ty : arg_ty) : Type :=
+  match ty with 
+  | AT_base b => denote_base b 
+  | AT_term => term 
+  | AT_bind ty => eval_arg ty
+  end.
+
+Fixpoint eval_args (tys : list arg_ty) : Type :=
+  match tys with 
+  | [] => unit
+  | ty :: tys => eval_arg ty * eval_args tys
+  end. 
+
+Definition eval_kind (k : kind) : Type :=
+  match k with 
+  | Kt => term
+  | Ka ty => eval_arg ty
+  | Kal tys => eval_args tys
+  end.
+
+Definition eval_ctor (c : ctor) : eval_args (ctor_type c) -> term :=
+  match c return eval_args (ctor_type c) -> term with 
+  | CApp => fun '(t1, (t2, _)) => App t1 t2 
+  | CLam => fun '(str, (t, _)) => Lam str t
+  end.
+
+Fixpoint eval {k} (t : O.expr k) : eval_kind k :=
+  match t in O.expr k0 return eval_kind k0 with 
+  | O.E_var i => Var i 
+  | O.E_ctor c al => eval_ctor c (eval al)
+  | O.E_al_nil => tt
+  | O.E_al_cons a al => (eval a, eval al)
+  | O.E_abase b x => x 
+  | O.E_aterm t => eval t 
+  | O.E_abind a => eval a
+  end. 
+
+Definition seval (s : O.subst) : subst :=
+  fun i => eval (s i).
+
+(** Push [eval] inside terms. *)
+
+Lemma eval_reify_inv (t : term) : 
+  eval (reify t) = t.
+Proof. induction t ; simpl ; f_equal ; auto. Qed.
+
+Lemma seval_sreify_inv (s : LevelZero.subst) :
+  seval (sreify s) =₁ s.
+Proof. intros i ; cbv [seval sreify]. now rewrite eval_reify_inv. Qed.
+
+Lemma eval_rename (t : O.expr Kt) (r : ren) :
+  eval (O.rename t r) = rename (eval t) r.
+Proof.
+revert t r. 
+apply (@term_ind' (fun (t : O.expr Kt) => forall r, eval (O.rename t r) = rename (eval t) r)).
+- intros i r. simpl. simp rename. simpl. reflexivity.
+- intros t1 t2 H1 H2 r. repeat (simp rename ; simpl). now rewrite H1, H2.
+- intros str t H r. repeat (simp rename ; simpl). now rewrite H.
+Qed.   
+
+Lemma eval_scons t s : 
+  seval (O.scons t s) =₁ scons (eval t) (seval s).
+Proof. intros [|i] ; reflexivity. Qed.
+
+Lemma eval_srcomp s r : 
+  seval (O.srcomp s r) =₁ srcomp (seval s) r.
+Proof. intros i. cbv [seval srcomp O.srcomp]. now rewrite eval_rename. Qed. 
+
+Lemma eval_up_subst s : 
+  seval (O.up_subst s) =₁ up_subst (seval s).
+Proof. 
+unfold O.up_subst, up_subst. rewrite eval_scons. simpl. 
+apply congr_scons ; [reflexivity|]. now rewrite eval_srcomp.
+Qed.
+
+Lemma eval_substitute (t : O.expr Kt) (s : O.subst) : 
+  eval (O.substitute t s) = substitute (eval t) (seval s).
+Proof.
+revert t s. 
+apply (@term_ind' (fun (t : O.expr Kt) => forall s, eval (O.substitute t s) = substitute (eval t) (seval s))).
+- intros i s. simpl. simp substitute. reflexivity.
+- intros t1 t2 H1 H2 s. repeat (simp substitute ; simpl). now rewrite H1, H2.
+- intros str t H s. repeat (simp substitute ; simpl). rewrite H. f_equal.
+  apply congr_substitute ; [reflexivity | now apply eval_up_subst].
+Qed.
+
+Lemma eval_scomp (s1 s2 : O.subst) :
+  seval (O.scomp s1 s2) =₁ scomp (seval s1) (seval s2).
+Proof. intros i. cbv [scomp O.scomp seval]. now rewrite eval_substitute. Qed.
+
+Lemma eval_rscomp (r : P.ren) (s : O.subst) :
+  seval (O.rscomp r s) =₁ rscomp r (seval s).
+Proof. reflexivity. Qed.
+
+(** Reification (Ltac). *)
+
+(** Returns [(t', p)] such that [p : eval t' = t]. *)
+Ltac2 rec reify (t : constr) : constr * constr :=
+  lazy_match! t with 
+  | Var ?i => constr:(O.E_var $i), constr:(@eq_refl _ (Var $i)) 
+  | App ?t1 ?t2 => 
+    let (t1', p1) := reify t1 in 
+    let (t2', p2) := reify t2 in 
+    let t' := constr:(
+      O.E_ctor CApp 
+        (O.E_al_cons (O.E_aterm $t1')
+        (O.E_al_cons (O.E_aterm $t2')
+         O.E_al_nil)))
+    in 
+    let p := constr:(congr_app $p1 $p2) in
+    (t', p)
+  | Lam ?str ?t1 =>
+    let (t1', p1) := reify t1 in
+    let t' := constr:(
+      O.E_ctor CLam 
+        (O.E_al_cons (O.E_abase BString $str)
+        (O.E_al_cons (O.E_abind (O.E_aterm $t1'))
+         O.E_al_nil)))
+    in 
+    let p := constr:(congr_lam $str $p1) in
+    (t', p)
+  | substitute ?t1 ?s =>
+    let (t1', p1) := reify t1 in 
+    let (s', p2) := reify_subst s in  
+    let t' := constr:(O.substitute $t1' $s') in
+    let p := constr:(
+      transitivity (eval_substitute $t1' $s') (congr_substitute $p1 $p2)) 
+    in
+    (t', p)
+  | ?t =>
+    let t' := constr:(reify $t) in 
+    let p := constr:(eval_reify_inv $t) in
+    (t', p)
+  end
+
+(** Returns [(s', p)] such that [p : seval s' =₁ s]. *)
+with reify_subst (s : constr) : constr * constr :=
+  lazy_match! s with 
+  | sshift => 
+    constr:(O.sshift), constr:(@reflexivity subst point_eq _ sshift)
+  | scons ?t ?s1 =>
+    let (t', p1) := reify t in 
+    let (s1', p2) := reify_subst s1 in 
+    let s' := constr:(O.scons $t' $s1') in 
+    let p := constr:(
+      transitivity (eval_scons $t' $s1') (congr_scons $p1 $p2)) 
+    in
+    (s', p)
+  | ?s => 
+    let s' := constr:(sreify $s) in 
+    let p := constr:(seval_sreify_inv $s) in 
+    (s', p)
+  end.
+
+(** Evaluation (Ltac). *)
+
+(** Returns [(t, p)] such that [p : eval t' = t]. *)
+Ltac2 rec eval (t' : constr) : constr * constr :=
+  lazy_match! t' with 
+  | O.E_var ?i => constr:(Var $i), constr:(@eq_refl _ (Var $i)) 
+  | O.substitute ?t' ?s' => 
+    let (t, p1) := eval t' in
+    let (s, p2) := eval_subst s' in 
+    constr:(substitute $t $s),
+    constr:(transitivity (eval_substitute $t' $s') (congr_substitute $p1 $p2))
+  | reify ?t => 
+    t, constr:(eval_reify_inv $t)
+  end
+
+(** Returns [(s, p)] such that [p : seval s' =₁ s]. *)
+with eval_subst (s' : constr) : constr * constr :=
+  lazy_match! s' with 
+  | O.scons ?t' ?s' =>
+    let (t, p1) := eval t' in 
+    let (s, p2) := eval_subst s' in 
+    constr:(LevelZero.scons $t $s),
+    constr:(transitivity (eval_scons $t' $s') (congr_scons $p1 $p2))
+  | O.scomp ?s1' ?s2' => 
+    let (s1, p1) := eval_subst s1' in 
+    let (s2, p2) := eval_subst s2' in
+    constr:(LevelZero.scomp $s1 $s2),
+    constr:(transitivity (eval_scomp $s1' $s2') (congr_scomp $p1 $p2))
+  | sreify ?s =>
+    s, constr:(seval_sreify_inv $s)
+  end.
+
+(** Testing. *)
+
+(*Axiom t_ax : term.
+
+Ltac2 Eval 
+  let (t', p) := reify constr:(substitute t_ax (scons (Var 0) sshift)) in 
+  constr:($p : eval $t' = substitute t_ax (scons (Var 0) sshift)).*)
+
+Axiom x t : term.
+Axiom s1 s2 : subst.
+
+(*Definition left := substitute (substitute t (up_subst s1)) (scons x s2).
+Definition right := substitute t (scons x (scomp s1 s2)).*)
+
+Definition left := substitute (substitute t (scons x s1)) s2.
+Definition right := substitute t (scons (substitute x s2) (scomp s1 s2)).
+
+From Ltac2 Require Import Printf.
+Import T.
+
+Ltac2 test_tac () : unit :=
+  lazy_match! Control.goal () with 
+  | @eq _ ?l0 ?r => 
+    (* Reify zero -> one. *)
+    let (l1, p) := reify l0 in
+    rewrite <-$p ; 
+    (* Reify one -> two. *)
+    let (e, l2) := reify_expr (empty_env ()) l1 in 
+    let e := build_env e in
+    change (eval (eeval $e $l2) = $r) ;
+    (* Simplify. *)
+    rewrite <-(esimp_sound $e $l2) ;
+    (* Eval two -> one. *)
+    cbv [seval eeval seval_functional eeval_functional
+         qeval reval qeval_functional reval_functional 
+         assign_ren assign_qnat assign_term assign_subst nth
+         esimp ssimp esimp_functional ssimp_functional 
+         substitute scomp substitute_functional scomp_functional sren
+         substitute_aux scomp_aux rsimp rsimp_functional qsimp_functional
+         sapply qsimp sapply_functional rscomp_functional 
+         sapply_aux] 
+  | _ => Control.throw_invalid_argument "not an equality"
+  end.
+
+Lemma test : left = right.
+Proof.
+unfold left, right.
+ltac2:(test_tac ()).
+ltac2:(
+  lazy_match! Control.goal () with 
+  | eval ?l1 = _ =>
+    let (_, p) := eval l1 in 
+    rewrite $p
+  end).
+Admitted.
